AReg.thy
@@ -16,7 +16,7 @@ step[intro!]:"x \<in> r \<and> y \<in> star r \<Longrightarrow> x@y \<in> star r
 primrec sem_reg :: "('v) regexp => 'v set\<Rightarrow> 'v list set" where 
 "sem_reg ESet v = {}"| (*Empty Set*)
 (*"sem_reg EString v = {[]}"| (*Empty String*)*)
-"sem_reg (Dot) vset = (λu. [u]) ` vset" | 
+"sem_reg (Dot) vset = (\<lambda>x .[x]) ` vset" | 
 "sem_reg (Concat r1 r2) v =(λu. fst u @ snd u) ` (sem_reg r1 v × sem_reg r2 v)"|
 "sem_reg (LChr a) v = {[a]}"|
 "sem_reg (v1||v2) a = (sem_reg v1 a) \<union> (sem_reg v2 a)"|
